Sodium.lean
@@ -1,15 +1,4 @@
--- This module serves as the root of the `Sodium` library.
--- Import modules here that should be built as part of the library.
 import «Sodium».Crypto.Monad
 import «Sodium».Crypto.Box
 import «Sodium».Crypto.SecretBox
-
-open Lean Sodium Crypto SecretBox
-
-#eval show CoreM Unit from do
-  CryptoM.toCoreM fun _ => do
-    let key ← mkSubKey
-    let cipher ← encrypt key "hello world"
-    println! cipher.bytes.toBase64
-    let .ok msg := ← decrypt key cipher | return ()
-    println! (msg : String)
+import «Sodium».Crypto.Session
