Sodium/Crypto/Session.lean
@@ -1,0 +1,92 @@
+import Sodium.Crypto.Monad
+
+open Lean
+
+namespace Sodium.Crypto
+
+open FFI KeyExch
+
+def SessionSpec : Spec where
+  name := `session.curve25519
+  seedBytes := SEEDBYTES
+  publicKeyBytes := PUBLICKEYBYTES
+  secretKeyBytes := SECRETKEYBYTES
+  sessionKeyBytes := SESSIONKEYBYTES
+
+variable {σ : Type} {τ : Sodium σ}
+
+@[simp]
+theorem session_meta_secret_key_compat :
+    ∀ key : SecretKey τ MetaSpec, key.bytes.size = SessionSpec.secretKeyBytes := by
+  intro k
+  exact k.size_eq_secret_key_bytes
+
+@[simp]
+theorem session_meta_public_key_compat :
+    ∀ key : PublicKey MetaSpec, key.bytes.size = SessionSpec.publicKeyBytes := by
+  intro k
+  exact k.size_eq_public_key_bytes
+
+@[simp]
+theorem session_meta_session_key_compat :
+    ∀ key : SessionKey τ MetaSpec, key.bytes.size = SessionSpec.sessionKeyBytes := by
+  intro k
+  exact k.size_eq_session_key_bytes
+
+@[simp]
+theorem session_meta_seed_compat :
+    ∀ key : Seed τ MetaSpec, key.bytes.size = SessionSpec.seedBytes := by
+  intro k
+  exact k.size_eq_seed_bytes
+
+instance : MetaSpecSupport PublicKey SessionSpec where
+  withSpec x := ⟨x.bytes, by exact x.size_eq_public_key_bytes⟩
+  liftSpec x := ⟨x.bytes, by simp⟩
+
+instance : MetaSpecSupport (SecretKey τ) SessionSpec where
+  withSpec x := ⟨x.bytes, by exact x.size_eq_secret_key_bytes⟩
+  liftSpec x := ⟨x.bytes, by simp⟩
+
+instance : MetaSpecSupport (KeyPair τ) SessionSpec where
+  withSpec x := ⟨withSpec x.public, withSpec x.secret⟩
+  liftSpec x := ⟨liftSpec x.public, liftSpec x.secret⟩
+
+instance : MetaSpecSupport (SessionKey τ) SessionSpec where
+  withSpec x := ⟨x.bytes, by exact x.size_eq_session_key_bytes⟩
+  liftSpec x := ⟨x.bytes, by simp⟩
+
+instance : MetaSpecSupport (Session τ) SessionSpec where
+  withSpec x := ⟨withSpec x.rx, withSpec x.tx⟩
+  liftSpec x := ⟨liftSpec x.rx, liftSpec x.tx⟩
+
+instance : MetaSpecSupport (Seed τ) SessionSpec where
+  withSpec x := ⟨x.bytes, by exact x.size_eq_seed_bytes⟩
+  liftSpec x := ⟨x.bytes, by simp⟩
+
+def mkFreshKeyPair : CryptoM τ (KeyPair τ SessionSpec) := do
+  let (pub, sec) ← keypair τ
+  if h : pub.size = SessionSpec.publicKeyBytes ∧ sec.size = SessionSpec.secretKeyBytes then
+    return ⟨⟨pub, h.1⟩, ⟨sec, h.2⟩⟩
+  else throwInvariantFailure
+
+def mkStaleKeyPair (seed : Seed τ SessionSpec) : CryptoM τ (KeyPair τ SessionSpec) := do
+  let (pub, sec) ← seedKeypair τ seed.bytes
+  if h : pub.size = SessionSpec.publicKeyBytes ∧ sec.size = SessionSpec.secretKeyBytes then
+    return ⟨⟨pub, h.1⟩, ⟨sec, h.2⟩⟩
+  else throwInvariantFailure
+
+def newServerSession? (keys : KeyPair τ SessionSpec) (client : PeerId SessionSpec) : CryptoM τ (Option (Session τ SessionSpec)) := do
+  let some (rx, tx) ← serverSessionKeys τ keys.public.bytes keys.secret.bytes client.pkey.bytes
+    | return none
+  if h : rx.size = SessionSpec.sessionKeyBytes ∧ tx.size = SessionSpec.sessionKeyBytes then
+    return some ⟨⟨rx, h.1⟩, ⟨tx, h.2⟩⟩
+  else throwInvariantFailure
+
+def newClientSession? (keys : KeyPair τ SessionSpec) (server : PeerId SessionSpec) : CryptoM τ (Option (Session τ SessionSpec)) := do
+  let some (rx, tx) ← clientSessionKeys τ keys.public.bytes keys.secret.bytes server.pkey.bytes
+    | return none
+  if h : rx.size = SessionSpec.sessionKeyBytes ∧ tx.size = SessionSpec.sessionKeyBytes then
+    return some ⟨⟨rx, h.1⟩, ⟨tx, h.2⟩⟩
+  else throwInvariantFailure
+
+end Sodium.Crypto
