Tests.lean
@@ -3,7 +3,10 @@ import Tests.EntropyArray
 import Tests.EntropyExtraction
 import Tests.SecureArray
 import Tests.SecureArrayComparison
+import Tests.SecureFileLoad
+import Tests.SecureFileStore
 import Tests.Box
 import Tests.SecretBox
+import Tests.KeyExch
 import Tests.ByteArray
--- import Tests.KeyDeriv  -- Needs API updates
+import Tests.KeyDeriv
